ArkLib.lean
@@ -289,11 +289,16 @@ import ArkLib.OracleReduction.Cast
 import ArkLib.OracleReduction.Composition.Parallel.Basic
 import ArkLib.OracleReduction.Composition.Sequential.Append
 import ArkLib.OracleReduction.Composition.Sequential.Append.Basic
+import ArkLib.OracleReduction.Composition.Sequential.Append.Completeness
 import ArkLib.OracleReduction.Composition.Sequential.Append.Execution
+import ArkLib.OracleReduction.Composition.Sequential.Append.OneMessage
+import ArkLib.OracleReduction.Composition.Sequential.Append.RoundByRound
 import ArkLib.OracleReduction.Composition.Sequential.Append.Security
 import ArkLib.OracleReduction.Composition.Sequential.Append.Simulation
 import ArkLib.OracleReduction.Composition.Sequential.Append.StateFunction
+import ArkLib.OracleReduction.Composition.Sequential.Completeness
 import ArkLib.OracleReduction.Composition.Sequential.General
+import ArkLib.OracleReduction.Composition.Sequential.GuardedCompleteness
 import ArkLib.OracleReduction.Composition.Sequential.IsPure
 import ArkLib.OracleReduction.Equiv
 import ArkLib.OracleReduction.Execution
